# trigonometric-formulas

Computation with some trigonometric formulas with $\sin()$, $\cos()$, $\tan()$, $\cot()$ from [Book 1](./Buch1.md).


* [Formula 1](./formulas/formula1/README.md)
```math
\sin^{2}\alpha + \cos^{2}\alpha = 1
```
* [Formula 2](./formulas/formula2/README.md)
```math
\tan{\alpha} = \frac{\sin\alpha}{\cos\alpha}
```
* [Formula 3](./formulas/formula3/README.md)
```math
\cot{\alpha} = \frac{\cos\alpha}{\sin\alpha}
```
* [Formula 4](./formulas/formula4/README.md)
```math
1 + \tan^{2}{\alpha} = \frac{1}{\cos^{2}{\alpha}}
```
* [Formula 5](./formulas/formula5/README.md)
```math
1 + \cot^{2}{\alpha} = \frac{1}{\sin^{2}{\alpha}}
```
* [Formula 6](./formulas/formula6/README.md)
```math
\sin{(\alpha + \beta)} = \sin{\alpha}\cos{\beta} + \cos{\alpha}\sin{\beta}
```
* [Formula 7](./formulas/formula7/README.md)
```math
\sin{(\alpha - \beta)} = \sin{\alpha}\cos{\beta} - \cos{\alpha}\sin{\beta}
```
* [Formula 8](./formulas/formula8/README.md)
```math
\cos{(\alpha + \beta)} = \cos{\alpha}\cos{\beta} - \sin{\alpha}\sin{\beta}
```
* [Formula 9](./formulas/formula9/README.md)
```math
\cos{(\alpha - \beta)} = \cos{\alpha}\cos{\beta} + \sin{\alpha}\sin{\beta}
```
* [Formula 10](./formulas/formula10/README.md)
```math
\tan{(\alpha + \beta)} = \frac{\tan{\alpha} + \tan{\beta}}{1 - \tan{\alpha}\tan{\beta}}
```
* [Formula 11](./formulas/formula11/README.md)
```math
\tan{(\alpha - \beta)} = \frac{\tan{\alpha} - \tan{\beta}}{1 + \tan{\alpha}\tan{\beta}}
```
* [Formula 12](./formulas/formula12/README.md)
```math
\cot{(\alpha + \beta)} = \frac{\cot{\alpha}\cot{\beta} - 1}{\cot{\beta} + \cot{\alpha}}
```
* [Formula 13](./formulas/formula13/README.md)
```math
\cot{(\alpha - \beta)} = \frac{\cot{\alpha}\cot{\beta} + 1}{\cot{\beta} - \cot{\alpha}}
```
* [Formula 14](./formulas/formula14/README.md)
```math
\sin{(\alpha + \beta)}\sin{(\alpha - \beta)} = \cos^{2}{\beta} - \cos^{2}{\alpha}
```
* [Formula 15](./formulas/formula15/README.md)
```math
\cos{(\alpha + \beta)}\cos{(\alpha - \beta)} = \cos^{2}{\beta} - \sin^{2}{\alpha}
```
* [Formula 16](./formulas/formula16/README.md)
```math
\sin{\alpha} = \pm\sqrt{1 - \cos^{2}{\alpha}}
```
* [Formula 17](./formulas/formula17/README.md)
```math
\sin{\alpha} = \pm\frac{\tan{\alpha}}{\sqrt{1 + \tan^{2}{\alpha}}}
```
* [Formula 18](./formulas/formula18/README.md)
```math
\sin{\alpha} = \pm\frac{1}{\sqrt{1 + \cot^{2}{\alpha}}}
```
* [Formula 19](./formulas/formula19/README.md)
```math
\cos{\alpha} = \pm\sqrt{1 - \sin^{2}{\alpha}}
```
* [Formula 20](./formulas/formula20/README.md)
```math
\cos{\alpha} = \pm\frac{1}{\sqrt{1 + \tan^{2}{\alpha}}}
```
* [Formula 21](./formulas/formula21/README.md)
```math
\cos{\alpha} = \pm\frac{\cot{\alpha}}{\sqrt{1 + \cot^{2}{\alpha}}}
```
* [Formula 22](./formulas/formula22/README.md)
```math
\tan{\alpha} = \pm\frac{\sin{\alpha}}{\sqrt{1 - \sin^{2}{\alpha}}}
```
* [Formula 23](./formulas/formula23/README.md)
```math
\tan{\alpha} = \pm\frac{\sqrt{1 - \cos^{2}{\alpha}}}{\cos{\alpha}}
```
* [Formula 24](./formulas/formula24/README.md)
```math
\cot{\alpha} = \pm\frac{\sqrt{1 - \sin^{2}{\alpha}}}{\sin{\alpha}}
```
* [Formula 25](./formulas/formula25/README.md)
```math
\cot{\alpha} = \pm\frac{\cos{\alpha}}{\sqrt{1 - \cos^{2}{\alpha}}}
```
* [Formula 26](./formulas/formula26/README.md)
```math
\sin{2\alpha} = 2\sin{\alpha}\cos{\alpha}
```
* [Formula 27](./formulas/formula27/README.md)
```math
\cos{2\alpha} = \cos^{2}{\alpha} - \sin^{2}{\alpha}
```
* [Formula 28](./formulas/formula28/README.md)
```math
\cos{2\alpha} = 1 - 2\sin^{2}{\alpha}
```
* [Formula 29](./formulas/formula29/README.md)
```math
\cos{2\alpha} = 2\cos^{2}{\alpha} - 1
```
* [Formula 30](./formulas/formula30/README.md)
```math
\tan{2\alpha} = \frac{2\tan{\alpha}}{1 - \tan^{2}{\alpha}}
```
* [Formula 31](./formulas/formula31/README.md)
```math
\tan{2\alpha} = \frac{2}{\cot{\alpha} - \tan{\alpha}}
```
* [Formula 32](./formulas/formula32/README.md)
```math
\cot{2\alpha} = \frac{\cot^{2}{\alpha} - 1}{2\cot{\alpha}}
```
* [Formula 33](./formulas/formula33/README.md)
```math
\cot{2\alpha} = \frac{\cot{\alpha} - \tan{\alpha}}{2}
```
* [Formula 34](./formulas/formula34/README.md)
```math
\sin{\alpha} = 2\sin{\frac{\alpha}{2}}\cos{\frac{\alpha}{2}}
```
* [Formula 35](./formulas/formula35/README.md)
```math
\cos{\alpha} = \cos^{2}{\frac{\alpha}{2}} - \sin^{2}{\frac{\alpha}{2}}
```
* [Formula 36](./formulas/formula36/README.md)
```math
\cos{\alpha} = 1 - 2\sin^{2}{\frac{\alpha}{2}}
```
* [Formula 37](./formulas/formula37/README.md)
```math
\cos{\alpha} = 2\cos^{2}{\frac{\alpha}{2}} - 1
```
* [Formula 38](./formulas/formula38/README.md)
```math
\tan{\alpha} = \frac{2\tan{\frac{\alpha}{2}}}{1 - \tan^{2}{\frac{\alpha}{2}}}
```
* [Formula 39](./formulas/formula39/README.md)
```math
\tan{\alpha} = \frac{2}{\cot{\frac{\alpha}{2}} - \tan{\frac{\alpha}{2}}}
```
* [Formula 40](./formulas/formula40/README.md)
```math
\cot{\alpha} = \frac{\cot^{2}{\frac{\alpha}{2}} - 1}{2\cot{\frac{\alpha}{2}}}
```
* [Formula 41](./formulas/formula41/README.md)
```math
\cot{\alpha} = \frac{\cot{\frac{\alpha}{2}} - \tan{\frac{\alpha}{2}}}{2}
```
* [Formula 42](./formulas/formula42/README.md)
```math
\sin{\frac{\alpha}{2}} = \sqrt{\frac{1 - \cos{\alpha}}{2}}
```
* [Formula 43](./formulas/formula43/README.md)
```math
\cos{\frac{\alpha}{2}} = \sqrt{\frac{1 + \cos{\alpha}}{2}}
```
* [Formula 44](./formulas/formula44/README.md)
```math
\tan{\frac{\alpha}{2}} = \sqrt{\frac{1 - \cos{\alpha}}{1 + \cos{\alpha}}}
```
* [Formula 45](./formulas/formula45/README.md)
```math
\tan{\frac{\alpha}{2}} = \frac{1 - \cos{\alpha}}{\sin{\alpha}}
```
* [Formula 46](./formulas/formula46/README.md)
```math
\tan{\frac{\alpha}{2}} = \frac{\sin{\alpha}}{1 + \cos{\alpha}}
```
* [Formula 47](./formulas/formula47/README.md)
```math
\cot{\frac{\alpha}{2}} = \sqrt{\frac{1 + \cos{\alpha}}{1 - \cos{\alpha}}}
```
* [Formula 48](./formulas/formula48/README.md)
```math
\cot{\frac{\alpha}{2}} = \frac{1 + \cos{\alpha}}{\sin{\alpha}}
```
* [Formula 49](./formulas/formula49/README.md)
```math
\cot{\frac{\alpha}{2}} = \frac{\sin{\alpha}}{1 - \cos{\alpha}}
```
* [Formula 50](./formulas/formula50/README.md)
```math
\sin{\alpha} = \sqrt{\frac{1 - \cos{2\alpha}}{2}}
```
* [Formula 51](./formulas/formula51/README.md)
```math
\sin{\alpha} = \sqrt{\frac{1 - \cos{2\alpha}}{2}}
```
* [Formula 52](./formulas/formula52/README.md)
```math
\cos{\alpha} = \sqrt{\frac{1 + \cos{2\alpha}}{2}}
```
* [Formula 53](./formulas/formula53/README.md)
```math
\tan{\alpha} = \sqrt{\frac{1 - \cos{2\alpha}}{1 + \cos{2\alpha}}}
```
* [Formula 54](./formulas/formula54/README.md)
```math
\tan{\alpha} = \frac{1 - \cos{2\alpha}}{\sin{2\alpha}}
```
* [Formula 55](./formulas/formula55/README.md)
```math
\cot{\alpha} = \sqrt{\frac{1 + \cos{2\alpha}}{1 - \cos{2\alpha}}}
```
* [Formula 56](./formulas/formula56/README.md)
```math
\cot{\alpha} = \frac{\sin{2\alpha}}{1 - \cos{2\alpha}}
```
* [Formula 57](./formulas/formula57/README.md)
```math
\cot{\alpha} = \frac{1 + \cos{2\alpha}}{\sin{2\alpha}}
```
* [Formula 58](./formulas/formula58/README.md)
```math
\sin{(3\alpha)} = 3\sin{\alpha} - 4\sin^3{\alpha}
```
* [Formula 59](./formulas/formula59/README.md)
```math
\sin{(4\alpha)} = 8\sin{\alpha}\cos^3{\alpha} - 4\sin{\alpha}\cos{\alpha}
```
* [Formula 60](./formulas/formula60/README.md)
```math
\sin{(5\alpha)} = 16\sin{\alpha}\cos^4{\alpha} - 12\sin{\alpha}\cos^2{\alpha} + \sin{\alpha}
```
* [Formula 61](./formulas/formula61/README.md)
```math
\cos{(3\alpha)} = 4\cos^3{\alpha} - 3\cos{\alpha}
```
* [Formula 62](./formulas/formula62/README.md)
```math
\cos{(4\alpha)} = 8\cos^4{\alpha} - 8\cos^2{\alpha} + 1
```
* [Formula 63](./formulas/formula63/README.md)
```math
\cos{(5\alpha)} = 16\cos^5{\alpha} - 20\cos^3{\alpha} + 5\cos{\alpha}
```
* [Formula 64](./formulas/formula64/README.md)
```math
\tan{(3\alpha)} = \frac{3\tan{\alpha} - \tan^3{\alpha}}{1 - 3\tan^2{\alpha}}
```
* [Formula 65](./formulas/formula65/README.md)
```math
\tan{(4\alpha)} = \frac{4\tan{\alpha} - 4\tan^3{\alpha}}{1 - 6\tan^2{\alpha} + \tan^4{\alpha}}
```
* [Formula 66](./formulas/formula66/README.md)
```math
\cot{(3\alpha)} = \frac{\cot^3{\alpha} - 3\cot{\alpha}}{3\cot^2{\alpha} - 1}
```
* [Formula 67](./formulas/formula67/README.md)
```math
\cot{(4\alpha)} = \frac{\cot^4{\alpha} - 6\cot^2{\alpha} + 1}{4\cot^3{\alpha} - 4\cot{\alpha}}
```
* [Formula 68](./formulas/formula68/README.md)
```math
\sin{\alpha} + \sin{\beta} = 2 \sin{\frac{\alpha + \beta}{2}} \cos{\frac{\alpha - \beta}{2}}
```
* [Formula 69](./formulas/formula69/README.md)
```math
\sin{\alpha} - \sin{\beta} = 2 \cos{\frac{\alpha + \beta}{2}} \sin{\frac{\alpha - \beta}{2}}
```
* [Formula 70](./formulas/formula70/README.md)
```math
\cos{\alpha} + \cos{\beta} = 2 \cos{\frac{\alpha + \beta}{2}} \cos{\frac{\alpha - \beta}{2}}
```
* [Formula 71](./formulas/formula71/README.md)
```math
\cos{\alpha} - \cos{\beta} = -2 \sin{\frac{\alpha + \beta}{2}} \sin{\frac{\alpha - \beta}{2}}
```
* [Formula 72](./formulas/formula72/README.md)
```math
\tan{\alpha} + \tan{\beta} = \frac{\sin{(\alpha + \beta)}}{\cos{\alpha}\cos{\beta}}
```
* [Formula 73](./formulas/formula73/README.md)
```math
\tan{\alpha} - \tan{\beta} = \frac{\sin{(\alpha - \beta)}}{\cos{\alpha}\cos{\beta}}
```
* [Formula 74](./formulas/formula74/README.md)
```math
\cot{\alpha} + \cot{\beta} = \frac{\sin{(\alpha + \beta)}}{\sin{\alpha}\sin{\beta}}
```
* [Formula 75](./formulas/formula75/README.md)
```math
\cot{\alpha} - \cot{\beta} = \frac{\sin{(\beta - \alpha)}}{\sin{\alpha}\sin{\beta}}
```
* [Formula 76](./formulas/formula76/README.md)
```math
\cos{\alpha} + \sin{\alpha} = \sqrt{2} \sin{(45^\circ + \alpha)}
```
* [Formula 77](./formulas/formula77/README.md)
```math
\cos{\alpha} + \sin{\alpha} = \sqrt{2} \cos{(45^\circ - \alpha)}
```
* [Formula 78](./formulas/formula78/README.md)
```math
\sqrt{2} \sin{(45^\circ + \alpha)} = \sqrt{2} \cos{(45^\circ - \alpha)}
```
* [Formula 79](./formulas/formula79/README.md)
```math
\cos{\alpha} - \sin{\alpha} = \sqrt{2} \sin{(45^\circ - \alpha)}
```
* [Formula 80](./formulas/formula80/README.md)
```math
\cos{\alpha} - \sin{\alpha} = \sqrt{2} \cos{(45^\circ + \alpha)}
```
* [Formula 81](./formulas/formula81/README.md)
```math
\sqrt{2} \sin{(45^\circ - \alpha)} = \sqrt{2} \cos{(45^\circ + \alpha)}
```
* [Formula 82](./formulas/formula82/README.md)
```math
\sin{\alpha} \sin{\beta} = \frac{1}{2} (\cos{(\alpha - \beta)} - \cos{(\alpha + \beta)})
```
* [Formula 83](./formulas/formula83/README.md)
```math
\cos{\alpha} \cos{\beta} = \frac{1}{2} (\cos{(\alpha - \beta)} + \cos{(\alpha + \beta)})
```
* [Formula 84](./formulas/formula84/README.md)
```math
\sin{\alpha} \cos{\beta} = \frac{1}{2} (\sin{(\alpha + \beta)} + \sin{(\alpha - \beta)})
```
* [Formula 85](./formulas/formula85/README.md)
```math
\cos{\alpha} \sin{\beta} = \frac{1}{2} (\sin{(\alpha + \beta)} - \sin{(\alpha - \beta)})
```
* [Formula 86](./formulas/formula86/README.md)
```math
\tan{\alpha} \tan{\beta} = \frac{\tan{\alpha} + \tan{\beta}}{\cot{\alpha} + \cot{\beta}}
```
* [Formula 87](./formulas/formula87/README.md)
```math
\tan{\alpha} \tan{\beta} = -\frac{\tan{\alpha} - \tan{\beta}}{\cot{\alpha} - \cot{\beta}}
```
* [Formula 88](./formulas/formula88/README.md)
```math
\cot{\alpha} \cot{\beta} = \frac{\cot{\alpha} + \cot{\beta}}{\tan{\alpha} + \tan{\beta}}
```
* [Formula 89](./formulas/formula89/README.md)
```math
\cot{\alpha} \cot{\beta} = -\frac{\cot{\alpha} - \cot{\beta}}{\tan{\alpha} - \tan{\beta}}
```
* [Formula 90](./formulas/formula90/README.md)
```math
\tan{\alpha} \cot{\beta} = \frac{\tan{\alpha} + \cot{\beta}}{\cot{\alpha} + \tan{\beta}}
```
* [Formula 91](./formulas/formula91/README.md)
```math
\tan{\alpha} \cot{\beta} = -\frac{\tan{\alpha} - \cot{\beta}}{\cot{\alpha} - \tan{\beta}}
```
* [Formula 92](./formulas/formula92/README.md)
```math
\cot{\alpha} \tan{\beta} = \frac{\cot{\alpha} + \tan{\beta}}{\tan{\alpha} + \cot{\beta}}
```
* [Formula 93](./formulas/formula93/README.md)
```math
\cot{\alpha} \tan{\beta} = -\frac{\cot{\alpha} - \tan{\beta}}{\tan{\alpha} - \cot{\beta}}
```
* [Formula 94](./formulas/formula94/README.md)
```math
\sin{\alpha} \sin{\beta} \sin{\gamma} = \frac{1}{4} (\sin{(\alpha + \beta - \gamma)} + \sin{(\beta + \gamma - \alpha)} + \sin{(\gamma + \alpha - \beta)} - \sin{(\alpha + \beta + \gamma)})
```
* [Formula 95](./formulas/formula95/README.md)
```math
\cos{\alpha} \cos{\beta} \cos{\gamma} = \frac{1}{4} (\cos{(\alpha + \beta - \gamma)} + \cos{(\beta + \gamma - \alpha)} + \cos{(\gamma + \alpha - \beta)} + \cos{(\alpha + \beta + \gamma)})
```
* [Formula 96](./formulas/formula96/README.md)
```math
\sin{\alpha} \sin{\beta} \cos{\gamma} = \frac{1}{4} (-\cos{(\alpha + \beta - \gamma)} + \cos{(\beta + \gamma - \alpha)} + \cos{(\gamma + \alpha - \beta)} - \cos{(\alpha + \beta + \gamma)})
```
